src/promotion/Promotion.v
@@ -46,7 +46,7 @@ Module Promotion.
       (PROMOTION: exists st_src lc_src st_tgt lc_tgt,
           <<FIND_SRC: IdentMap.find p c_src.(Configuration.threads) = Some (existT _ lang st_src, lc_src)>> /\
           <<FIND_TGT: IdentMap.find p c_tgt.(Configuration.threads) = Some (existT _ lang st_tgt, lc_tgt)>> /\
-          <<SIM_THREAD: SimThreadPromotion.sim_thread_reserve
+          <<SIM_THREAD: SimThreadPromotion.sim_thread_all
                           l r
                           (Thread.mk lang st_src lc_src c_src.(Configuration.sc) c_src.(Configuration.memory))
                           (Thread.mk lang st_tgt lc_tgt c_tgt.(Configuration.sc) c_tgt.(Configuration.memory))>>)
@@ -99,7 +99,28 @@ Module Promotion.
       dup SIM. inv SIM0. des. ss.
       dup WF_SRC. inv WF_SRC0. inv WF.
       exploit THREADS; eauto. i. clear DISJOINT THREADS.
-      exploit SimThreadPromotion.step_reserve_sim_thread; try exact SIM_THREAD; eauto. i. des.
+      inv SIM_THREAD.
+      { esplits; eauto. ii. destruct (Ident.eq_dec tid p).
+        + subst. rewrite FIND in FIND_SRC0. Configuration.simplify2.
+          exploit TERMINAL_TGT; eauto. i. des.
+          split.
+          * exploit SimThreadPromotion.sim_thread_terminal; eauto.
+          * inv THREAD. unnw. econs.
+            exploit SimThreadPromotion.sim_thread_promises_bot; eauto.
+        + clear st_src lc_src st_tgt lc_tgt x FIND_SRC0 FIND_TGT0 H SC MEM.
+          exploit sim_conf_find; eauto. i. des.
+          exploit x0; eauto. i. des.
+          exploit FIND_SRC; eauto. i. subst.
+          exploit FIND_TGT; eauto. i. subst.
+          clear x0 x1 FIND_SRC FIND_TGT.
+          exploit sim_conf_sim_thread_other; eauto. intro SIM_THREAD.
+          exploit TERMINAL_TGT; eauto. i. des.
+          split.
+          * exploit SimThreadOther.sim_thread_terminal; eauto.
+          * inv THREAD. unnw. econs.
+            exploit SimThreadOther.sim_thread_promises_bot; eauto.
+      }
+      exploit SimThreadPromotion.step_reserve_sim_thread; try exact H; eauto. i. des.
       destruct e2_src.
       esplits.
       - econs 2; eauto. econs.
@@ -118,7 +139,7 @@ Module Promotion.
             exploit SimThreadPromotion.sim_thread_promises_bot; eauto.
         + Configuration.simplify2.
           clear st_src lc_src st_tgt lc_tgt x from to state local sc memory
-                FIND_SRC0 FIND_TGT0 SIM_THREAD SC MEM STEP SIM2.
+                FIND_SRC0 FIND_TGT0 H SC MEM STEP SIM2.
           exploit sim_conf_find; eauto. i. des.
           exploit x0; eauto. i. des.
           exploit FIND_SRC; eauto. i. subst.
@@ -143,7 +164,7 @@ Module Promotion.
       exploit THREADS; eauto. intro WF1_SRC. clear DISJOINT THREADS.
       dup WF_TGT. inv WF_TGT0. inv WF. ss.
       exploit THREADS; eauto. intro WF1_TGT. clear DISJOINT THREADS.
-      exploit SimThreadPromotion.sim_thread_reserve_plus_step; eauto. s. i. des.
+      exploit SimThreadPromotion.sim_thread_all_plus_step; eauto; ss. s. i. des.
       destruct e_src; ss. inv STEP_SRC. destruct e3_src. ss.
       assert (CSTEP: Configuration.step
                        MachineEvent.failure p
@@ -178,7 +199,8 @@ Module Promotion.
         inv WF_SRC. inv WF. ss. exploit THREADS; eauto.
     }
 
-    { (* promotion: normal *)
+    destruct (classic (ThreadEvent.get_machine_event e0 = MachineEvent.silent)) eqn:SILENT.
+    { (* promotion: silent *)
       destruct c_src as [ths1_src sc1_src mem1_src].
       destruct c_tgt as [ths1_tgt sc1_tgt mem1_tgt].
       dup SIM. inv SIM0. des. ss.
@@ -188,7 +210,9 @@ Module Promotion.
       exploit THREADS; eauto. intro WF1_SRC. clear DISJOINT THREADS.
       dup WF_TGT. inv WF_TGT0. inv WF. ss.
       exploit THREADS; eauto. intro WF1_TGT. clear DISJOINT THREADS.
-      exploit SimThreadPromotion.sim_thread_reserve_plus_step; eauto. s. i. des.
+      exploit SimThreadPromotion.sim_thread_all_plus_step; eauto.
+      { destruct e0; ss. }
+      s. i. des.
       destruct e3_src. ss.
       assert (CSTEP: Configuration.opt_step
                        (ThreadEvent.get_machine_event e_src) p
@@ -221,6 +245,53 @@ Module Promotion.
       rewrite <- EVENT0. esplits; eauto.
       exploit Configuration.opt_step_future; try exact CSTEP; eauto. s. i. des.
       hexploit Thread.rtc_all_step_prev_None; try eapply Thread.tau_opt_all; eauto. s. i. des.
+      right. apply CIH. econs; ss.
+      - repeat rewrite Threads.tids_add.
+        repeat rewrite IdentSet.add_mem; ss.
+        + rewrite Threads.tids_o. rewrite TID. ss.
+        + rewrite Threads.tids_o. rewrite FIND_SRC0. ss.
+      - i. revert FIND. rewrite IdentMap.gsspec. condtac; ss; i.
+        + inv FIND. ss.
+        + inv SIM. eapply FIND_SRC; eauto.
+      - i. revert FIND. rewrite IdentMap.gsspec. condtac; ss; i.
+        + inv FIND. ss.
+        + inv SIM. eapply FIND_TGT; eauto.
+      - repeat rewrite IdentMap.gsspec. condtac; ss. esplits; eauto.
+      - i. revert FIND_SRC. rewrite IdentMap.gsspec. condtac; ss; i.
+        revert FIND_TGT. rewrite IdentMap.gsspec. condtac; ss; i.
+        exploit sim_conf_sim_thread_other; eauto. s. i.
+        eapply SimThreadOther.sim_thread_future; eauto; try apply SIM3.
+        inv WF_SRC. inv WF. ss. exploit THREADS; eauto.
+    }
+
+    { (* promotion: syscall *)
+      destruct c_src as [ths1_src sc1_src mem1_src].
+      destruct c_tgt as [ths1_tgt sc1_tgt mem1_tgt].
+      dup SIM. inv SIM0. des. ss.
+      clear FIND_SRC FIND_TGT OTHER.
+      rewrite TID in FIND_TGT0. Configuration.simplify2.
+      dup WF_SRC. inv WF_SRC0. inv WF. ss.
+      exploit THREADS; eauto. intro WF1_SRC. clear DISJOINT THREADS.
+      dup WF_TGT. inv WF_TGT0. inv WF. ss.
+      exploit THREADS; eauto. intro WF1_TGT. clear DISJOINT THREADS.
+      destruct e0; ss.
+      exploit SimThreadPromotion.sim_thread_all_plus_step_syscall; eauto. s. i. des.
+      destruct e3_src. ss.
+      assert (CSTEP: Configuration.opt_step
+                       (ThreadEvent.get_machine_event e_src) p
+                       (Configuration.mk ths1_src sc1_src mem1_src)
+                       (Configuration.mk
+                          (IdentMap.add p (existT (fun (lang: language) => lang.(Language.state)) lang state, local) ths1_src)
+                          sc memory)).
+      { econs 2. econs 2; eauto.
+        - ii. subst. ss.
+        - destruct e_src; ss. inv STEP_SRC; [inv STEP0|].
+          inv STEP0. inv LOCAL. inv LOCAL0. ss.
+          ii. right. esplits; eauto.
+      }
+      rewrite <- EVENT0. esplits; eauto.
+      exploit Configuration.opt_step_future; try exact CSTEP; eauto. s. i. des.
+      hexploit Thread.rtc_all_step_prev_None; try eapply Thread.tau_opt_all; [|econs 2|]; eauto. s. i. des.
       right. apply CIH. econs; ss.
       - repeat rewrite Threads.tids_add.
         repeat rewrite IdentSet.add_mem; ss.
@@ -283,7 +354,7 @@ Module Promotion.
         + inv SIM. eapply FIND_TGT; eauto.
       - repeat rewrite IdentMap.gsspec. condtac; try congr.
         inv SIM. des. ss. esplits; eauto.
-        eapply SimThreadPromotion.sim_thread_reserve_future; eauto; try apply SIM3.
+        eapply SimThreadPromotion.sim_thread_all_future; eauto; try apply SIM3.
         inv WF_SRC. inv WF. ss. exploit THREADS; eauto.
       - i. revert FIND_SRC. rewrite IdentMap.gsspec. condtac; ss; i.
         + subst. revert FIND_TGT. rewrite IdentMap.gsspec. condtac; ss; i. Configuration.simplify2.
@@ -353,7 +424,7 @@ Module Promotion.
         + inv SIM. eapply FIND_TGT; eauto.
       - repeat rewrite IdentMap.gsspec. condtac; try congr.
         inv SIM. des. ss. esplits; eauto.
-        eapply SimThreadPromotion.sim_thread_reserve_future; eauto; try apply SIM3.
+        eapply SimThreadPromotion.sim_thread_all_future; eauto; try apply SIM3.
         inv WF_SRC. inv WF. ss. exploit THREADS; eauto.
       - i. revert FIND_SRC. rewrite IdentMap.gsspec. condtac; ss; i.
         + subst. revert FIND_TGT. rewrite IdentMap.gsspec. condtac; ss; i. Configuration.simplify2.
@@ -404,142 +475,77 @@ Module Promotion.
           <<SYNTAX: syn_src = syn_tgt>>)
   .
 
-  Inductive sim_conf_init (p: Ident.t) (l: Loc.t) (r: Reg.t) (c_src c_tgt: Configuration.t): Prop :=
-  | sim_conf_init_intro
-      (TIDS: Threads.tids c_src.(Configuration.threads) = Threads.tids c_tgt.(Configuration.threads))
-      (FIND_SRC: forall tid lang_src st_src lc_src
-                   (FIND: IdentMap.find tid c_src.(Configuration.threads) = Some (existT _ lang_src st_src, lc_src)),
-          lang_src = lang)
-      (FIND_TGT: forall tid lang_tgt st_tgt lc_tgt
-                   (FIND: IdentMap.find tid c_tgt.(Configuration.threads) = Some (existT _ lang_tgt st_tgt, lc_tgt)),
-          lang_tgt = lang)
-      (PROMOTION: exists st_src lc_src st_tgt lc_tgt,
-          <<FIND_SRC: IdentMap.find p c_src.(Configuration.threads) = Some (existT _ lang st_src, lc_src)>> /\
-          <<FIND_TGT: IdentMap.find p c_tgt.(Configuration.threads) = Some (existT _ lang st_tgt, lc_tgt)>> /\
-          <<SIM_THREAD: SimThreadPromotion.sim_thread
-                          l r
-                          (Thread.mk lang st_src lc_src c_src.(Configuration.sc) c_src.(Configuration.memory))
-                          (Thread.mk lang st_tgt lc_tgt c_tgt.(Configuration.sc) c_tgt.(Configuration.memory))>>)
-      (OTHER: forall tid st_src lc_src st_tgt lc_tgt
-                (TID: tid <> p)
-                (FIND_SRC: IdentMap.find tid c_src.(Configuration.threads) = Some (existT _ lang st_src, lc_src))
-                (FIND_TGT: IdentMap.find tid c_tgt.(Configuration.threads) = Some (existT _ lang st_tgt, lc_tgt)),
-          <<SIM_THREAD: SimThreadOther.sim_thread
-                          l
-                          (Thread.mk lang st_src lc_src c_src.(Configuration.sc) c_src.(Configuration.memory))
-                          (Thread.mk lang st_tgt lc_tgt c_tgt.(Configuration.sc) c_tgt.(Configuration.memory))>>)
-  .
-  Hint Constructors sim_conf_init.
-
   Lemma init_sim_conf
         p l r program_src program_tgt
         (PROMOTE: promote_program p l r program_src program_tgt):
-    exists c_src,
-      <<STEP: Configuration.step MachineEvent.silent p (Configuration.init program_src) c_src>> /\
-      <<SIM: sim_conf p l r c_src (Configuration.init program_tgt)>>.
+    <<SIM: sim_conf p l r (Configuration.init program_src) (Configuration.init program_tgt)>>.
   Proof.
-    assert (INIT: sim_conf_init p l r (Configuration.init program_src) (Configuration.init program_tgt)).
-    { inv PROMOTE. econs; ss; i.
-      - apply IdentSet.ext. i.
-        repeat rewrite Threads.tids_o.
-        unfold Threads.init.
-        repeat rewrite IdentMap.Facts.map_o.
-        specialize (@syntax_tids_o i program_src). i.
-        specialize (@syntax_tids_o i program_tgt). i.
+    inv PROMOTE. econs; ss; i.
+    - apply IdentSet.ext. i.
+      repeat rewrite Threads.tids_o.
+      unfold Threads.init.
+      repeat rewrite IdentMap.Facts.map_o.
+      specialize (@syntax_tids_o i program_src). i.
+      specialize (@syntax_tids_o i program_tgt). i.
+      destruct (@UsualFMapPositive.UsualPositiveMap'.find
+                  (@sigT _ (@Language.syntax ProgramEvent.t)) i program_src) eqn:SRC;
         destruct (@UsualFMapPositive.UsualPositiveMap'.find
-                    (@sigT _ (@Language.syntax ProgramEvent.t)) i program_src) eqn:SRC;
-          destruct (@UsualFMapPositive.UsualPositiveMap'.find
-                      (@sigT _ (@Language.syntax ProgramEvent.t)) i program_tgt) eqn:TGT; ss.
-        + assert (@UsualFMapPositive.UsualPositiveMap'.find
-                    (@sigT _ (@Language.syntax ProgramEvent.t)) i program_src = IdentMap.find i program_src) by ss.
-          rewrite <- H1 in *. rewrite SRC in *. ss.
-          assert (@UsualFMapPositive.UsualPositiveMap'.find
-                    (@sigT _ (@Language.syntax ProgramEvent.t)) i program_tgt = IdentMap.find i program_tgt) by ss.
-          rewrite <- H2 in *. rewrite TGT in *. ss.
-          rewrite TIDS in *. congr.
-        + assert (@UsualFMapPositive.UsualPositiveMap'.find
-                    (@sigT _ (@Language.syntax ProgramEvent.t)) i program_src = IdentMap.find i program_src) by ss.
-          rewrite <- H1 in *. rewrite SRC in *. ss.
-          assert (@UsualFMapPositive.UsualPositiveMap'.find
-                    (@sigT _ (@Language.syntax ProgramEvent.t)) i program_tgt = IdentMap.find i program_tgt) by ss.
-          rewrite <- H2 in *. rewrite TGT in *. ss.
-          rewrite TIDS in *. congr.
-      - unfold Threads.init in *.
-        rewrite IdentMap.Facts.map_o in *.
-        destruct (@UsualFMapPositive.UsualPositiveMap'.find
-                    (@sigT _ (@Language.syntax ProgramEvent.t)) tid program_src) eqn:SRC; ss.
-        destruct s. ss. inv FIND. eapply FIND_SRC; eauto.
-      - unfold Threads.init in *.
-        rewrite IdentMap.Facts.map_o in *.
-        destruct (@UsualFMapPositive.UsualPositiveMap'.find
-                    (@sigT _ (@Language.syntax ProgramEvent.t)) tid program_tgt) eqn:SRC; ss.
-        destruct s. ss. inv FIND. eapply FIND_TGT; eauto.
-      - unfold Threads.init in *.
-        repeat rewrite IdentMap.Facts.map_o in *. des.
-        replace (@UsualFMapPositive.UsualPositiveMap'.find
-                   (@sigT _ (@Language.syntax ProgramEvent.t)) p program_src) with
-            (IdentMap.find p program_src) by ss.
-        replace (@UsualFMapPositive.UsualPositiveMap'.find
-                   (@sigT _ (@Language.syntax ProgramEvent.t)) p program_tgt) with
-            (IdentMap.find p program_tgt) by ss.
-        rewrite FIND_SRC0. rewrite FIND_TGT0. ss.
-        esplits; eauto.
-        unfold State.init. econs; ss; try refl.
-        + instantiate (1 := 0). left. econs; eauto. refl.
-        + ii. rewrite Memory.bot_get in *. ss.
-        + replace (Memory.max_ts l Memory.init) with Time.bot by ss.
-          unfold Memory.get, Memory.init, Cell.get, Cell.init, Cell.Raw.init. ss.
-          rewrite DOMap.singleton_eq. unfold Message.elt. eauto.
-        + i. rewrite Memory.bot_get. ss.
-        + ii. unfold Memory.get, Memory.init, Cell.get, Cell.init in GET.
-          apply DOMap.singleton_find_inv in GET. des. inv GET0.
-      - unfold Threads.init in *.
-        rewrite IdentMap.Facts.map_o in *.
-        destruct (@UsualFMapPositive.UsualPositiveMap'.find
-                    (@sigT _ (@Language.syntax ProgramEvent.t)) tid program_src) eqn:SRC;
-          destruct (@UsualFMapPositive.UsualPositiveMap'.find
-                      (@sigT _ (@Language.syntax ProgramEvent.t)) tid program_tgt) eqn:TGT; ss.
-        destruct s, s0; ss.  Configuration.simplify2.
-        exploit OTHER; eauto. i. des.
-        unfold State.init. econs; ss; try refl.
-        + f_equal. ss.
-        + i. rewrite Memory.bot_get. ss.
-        + ii. rewrite Memory.bot_get in *. ss.
-    }
-    inv INIT. des.
-    specialize (Configuration.init_wf program_src). intro WF_SRC.
-    specialize (Configuration.init_wf program_tgt). intro WF_TGT.
-    dup WF_SRC. inv WF_SRC0. inv WF.
-    exploit THREADS; eauto. intro WF_SRC1. clear DISJOINT THREADS.
-    dup WF_TGT. inv WF_TGT0. inv WF.
-    exploit THREADS; eauto. intro WF_TGT1. clear DISJOINT THREADS.
-    exploit SimThreadPromotion.step_sim_thread_reserve; eauto; ss. i. des.
-    destruct e2_src. ss.
-    exploit Thread.step_future; eauto. s. i. des.
-    esplits.
-    - replace MachineEvent.silent with
-          (ThreadEvent.get_machine_event (ThreadEvent.promise l from to Message.reserve Memory.op_kind_add)) by ss.
-      econs 2; eauto; ss.
-      eapply SimThreadPromotion.sim_thread_reserve_consistent; eauto. ii. ss.
-      right. esplits; eauto. ss.
-      unfold Threads.init in *.
+                    (@sigT _ (@Language.syntax ProgramEvent.t)) i program_tgt) eqn:TGT; ss.
+      + assert (@UsualFMapPositive.UsualPositiveMap'.find
+                  (@sigT _ (@Language.syntax ProgramEvent.t)) i program_src = IdentMap.find i program_src) by ss.
+        rewrite <- H1 in *. rewrite SRC in *. ss.
+        assert (@UsualFMapPositive.UsualPositiveMap'.find
+                  (@sigT _ (@Language.syntax ProgramEvent.t)) i program_tgt = IdentMap.find i program_tgt) by ss.
+        rewrite <- H2 in *. rewrite TGT in *. ss.
+        rewrite TIDS in *. congr.
+      + assert (@UsualFMapPositive.UsualPositiveMap'.find
+                  (@sigT _ (@Language.syntax ProgramEvent.t)) i program_src = IdentMap.find i program_src) by ss.
+        rewrite <- H1 in *. rewrite SRC in *. ss.
+        assert (@UsualFMapPositive.UsualPositiveMap'.find
+                  (@sigT _ (@Language.syntax ProgramEvent.t)) i program_tgt = IdentMap.find i program_tgt) by ss.
+        rewrite <- H2 in *. rewrite TGT in *. ss.
+        rewrite TIDS in *. congr.
+    - unfold Threads.init in *.
       rewrite IdentMap.Facts.map_o in *.
       destruct (@UsualFMapPositive.UsualPositiveMap'.find
-                  (@sigT _ (@Language.syntax ProgramEvent.t)) p program_tgt) eqn:TGT; ss.
-      destruct s; ss. Configuration.simplify2.
-    - econs; ss.
-      + repeat rewrite Threads.tids_add.
-        repeat rewrite IdentSet.add_mem; ss.
-        rewrite Threads.tids_o. rewrite FIND_SRC0. ss.
-      + i. revert FIND. rewrite IdentMap.gsspec. condtac; ss; i.
-        * inv FIND. ss.
-        * eauto.
-      + repeat rewrite IdentMap.gsspec. condtac; ss. esplits; eauto.
-      + i. revert FIND_SRC1. rewrite IdentMap.gsspec. condtac; ss; i.
-        exploit OTHER; eauto. i.
-        eapply SimThreadOther.sim_thread_future; eauto; try apply SIM2.
-        * inv WF_SRC. inv WF. ss. exploit THREADS; eauto.
-        * hexploit Thread.step_prev_None; eauto.
+                  (@sigT _ (@Language.syntax ProgramEvent.t)) tid program_src) eqn:SRC; ss.
+      destruct s. ss. inv FIND. eapply FIND_SRC; eauto.
+    - unfold Threads.init in *.
+      rewrite IdentMap.Facts.map_o in *.
+      destruct (@UsualFMapPositive.UsualPositiveMap'.find
+                  (@sigT _ (@Language.syntax ProgramEvent.t)) tid program_tgt) eqn:SRC; ss.
+      destruct s. ss. inv FIND. eapply FIND_TGT; eauto.
+    - unfold Threads.init in *.
+      repeat rewrite IdentMap.Facts.map_o in *. des.
+      replace (@UsualFMapPositive.UsualPositiveMap'.find
+                 (@sigT _ (@Language.syntax ProgramEvent.t)) p program_src) with
+          (IdentMap.find p program_src) by ss.
+      replace (@UsualFMapPositive.UsualPositiveMap'.find
+                 (@sigT _ (@Language.syntax ProgramEvent.t)) p program_tgt) with
+          (IdentMap.find p program_tgt) by ss.
+      rewrite FIND_SRC0. rewrite FIND_TGT0. ss.
+      esplits; eauto.
+      left. unfold State.init. econs; ss; try refl.
+      + instantiate (1 := 0). left. econs; eauto. refl.
+      + ii. rewrite Memory.bot_get in *. ss.
+      + replace (Memory.max_ts l Memory.init) with Time.bot by ss.
+        unfold Memory.get, Memory.init, Cell.get, Cell.init, Cell.Raw.init. ss.
+        rewrite DOMap.singleton_eq. unfold Message.elt. eauto.
+      + i. rewrite Memory.bot_get. ss.
+      + ii. unfold Memory.get, Memory.init, Cell.get, Cell.init in GET.
+        apply DOMap.singleton_find_inv in GET. des. inv GET0.
+    - unfold Threads.init in *.
+      rewrite IdentMap.Facts.map_o in *.
+      destruct (@UsualFMapPositive.UsualPositiveMap'.find
+                  (@sigT _ (@Language.syntax ProgramEvent.t)) tid program_src) eqn:SRC;
+        destruct (@UsualFMapPositive.UsualPositiveMap'.find
+                    (@sigT _ (@Language.syntax ProgramEvent.t)) tid program_tgt) eqn:TGT; ss.
+      destruct s, s0; ss.  Configuration.simplify2.
+      exploit OTHER; eauto. i. des.
+      unfold State.init. econs; ss; try refl.
+      + f_equal. ss.
+      + i. rewrite Memory.bot_get. ss.
+      + ii. rewrite Memory.bot_get in *. ss.
   Qed.
 
   Theorem promote_behavior
@@ -551,9 +557,7 @@ Module Promotion.
     exploit init_sim_conf; eauto. i. des.
     specialize (Configuration.init_wf program_src). intro WF_SRC.
     specialize (Configuration.init_wf program_tgt). intro WF_TGT.
-    exploit Configuration.step_future; eauto. i. des.
     hexploit sim_conf_sim; eauto. i.
-    exploit sim_adequacy; try exact H; eauto. i.
-    econs 4; eauto.
+    exploit sim_adequacy; try exact H; eauto.
   Qed.
 End Promotion.
